src/checker.lean
@@ -3,7 +3,6 @@ import expr
 
 namespace coc
 
-open idx
 open expr
 open ctx
 
@@ -16,7 +15,7 @@ def expr.as_pi : expr → string ⊕ (expr × expr)
 | e          := sum.inl $ "expression " ++ e.show ++ " is not a function"
 
 def ctx.try_nth : ctx → nat → string ⊕ expr
-| []       _       := sum.inl "undefined variable"
+| []       n       := sum.inl $ "variable index overflowed by " ++ to_string n
 | (t :: Γ) 0       := sum.inr t
 | (t :: Γ) (n + 1) := ctx.try_nth Γ n
 
@@ -25,30 +24,26 @@ def ctx.try_nth : ctx → nat → string ⊕ expr
     (2) Returns `sort (n + 1)` itself;
     (3) Returns a well-formed expression of type `sort 0`, representing the proposition it proves;
     (4) Returns `sort 0` itself. -/
-meta def expr.check_rec : expr → Π (Γ Δ : ctx), string ⊕ expr
-| (sort s)        Γ Δ := return (sort (s + 1))
-| (var (bound b)) Γ Δ := do t <- Δ.try_nth b, return (expr.shift t 0 (nat.succ b))
-| (var (free f))  Γ Δ := do t <- Γ.try_nth (Γ.length - 1 - f), return t
-| (app l r)   Γ Δ := do
-  { tl        ← l.check_rec Γ Δ,
+meta def expr.check : expr → Π (Γ : ctx), string ⊕ expr
+| (sort s)    Γ := return (sort (s + 1))
+| (var v)     Γ := do t <- Γ.try_nth v, return (t.shift 0 v.succ)
+| (app l r)   Γ := do
+  { tl        ← l.check Γ,
     ⟨t₁, t₂⟩  ← tl.as_pi,
-    tr        ← r.check_rec Γ Δ,
+    tr        ← r.check Γ,
     if t₁.reduce = tr.reduce
-    then return (expr.subst t₂ 0 r)
+    then return (t₂.subst 0 r)
     else sum.inl $ "argument type mismatch: " ++ t₁.show ++ " != " ++ tr.show }
-| (lam t e)   Γ Δ := do
-  { t'        ← t.check_rec Γ Δ,
+| (lam t e)   Γ := do
+  { t'        ← t.check Γ,
     _         ← t'.as_sort,
-    t₂        ← e.check_rec Γ (t :: Δ),
+    t₂        ← e.check (t :: Γ),
     return (pi t t₂) }
-| (pi t₁ t₂)  Γ Δ := do
-  { t'        ← t₁.check_rec Γ Δ,
+| (pi t₁ t₂)  Γ := do
+  { t'        ← t₁.check Γ,
     s₁        ← t'.as_sort,
-    t''       ← t₂.check_rec Γ (t₁ :: Δ),
+    t''       ← t₂.check (t₁ :: Γ),
     s₂        ← t''.as_sort,
     return (sort (max s₁ s₂)) }
-
-meta def expr.check (e : expr) (Γ : ctx) : string ⊕ expr :=
-  e.check_rec Γ []
 
 end coc
