src/main.lean
@@ -4,45 +4,38 @@ import checker
 namespace coc
 section
 
-open idx
 open expr
 open ctx
 
 -- Examples adapted from ApiMu (FOLContext).
-def bv := var ∘ bound
-def fv := var ∘ free
 def prop := sort 0
 def type := sort 1
 def bin := λ a f b, app (app f a) b
 
 def c₁ : ctx :=
-  [ (pi (fv 0) $ pi (fv 0) prop), -- [13] mem       : setvar → setvar → Prop
-    (pi (pi (fv 0) prop) prop),   -- [12] unique    : (setvar → Prop) → Prop
-    (pi (pi (fv 0) prop) prop),   -- [11] exists    : (setvar → Prop) → Prop
-    (pi (pi (fv 0) prop) prop),   -- [10] forall    : (setvar → Prop) → Prop
-    (pi prop $ pi prop prop),     -- [9]  iff       : Prop → Prop → Prop
-    (pi prop $ pi prop prop),     -- [8]  implies   : Prop → Prop → Prop
-    (pi prop $ pi prop prop),     -- [7]  or        : Prop → Prop → Prop
-    (pi prop $ pi prop prop),     -- [6]  and       : Prop → Prop → Prop
-    (pi prop prop),               -- [5]  not       : Prop → Prop
-    prop,                         -- [4]  false     : Prop
-    prop,                         -- [3]  true      : Prop
-    (pi (fv 0) $ pi (fv 0) prop), -- [2]  equals    : setvar → setvar → Prop
-    (fv 0),                       -- [1]  arbitrary : setvar
-    type ]                        -- [0]  setvar    : Type
-
-def and := fv 6
-def iff := fv 9
-def for := app (fv 10) ∘ lam (fv 0)
-def exi := app (fv 11) ∘ lam (fv 0)
-def mem := fv 13
+  [ (pi (var 12) $ pi (var 12) prop), -- [13] mem       : setvar → setvar → Prop
+    (pi (pi (var 11) prop) prop),     -- [12] unique    : (setvar → Prop) → Prop
+    (pi (pi (var 10) prop) prop),     -- [11] exists    : (setvar → Prop) → Prop
+    (pi (pi (var 9) prop) prop),      -- [10] forall    : (setvar → Prop) → Prop
+    (pi prop $ pi prop prop),         -- [9]  iff       : Prop → Prop → Prop
+    (pi prop $ pi prop prop),         -- [8]  implies   : Prop → Prop → Prop
+    (pi prop $ pi prop prop),         -- [7]  or        : Prop → Prop → Prop
+    (pi prop $ pi prop prop),         -- [6]  and       : Prop → Prop → Prop
+    (pi prop prop),                   -- [5]  not       : Prop → Prop
+    prop,                             -- [4]  false     : Prop
+    prop,                             -- [3]  true      : Prop
+    (pi (var 0) $ pi (var 0) prop),   -- [2]  equals    : setvar → setvar → Prop
+    (var 0),                          -- [1]  arbitrary : setvar
+    type ]                            -- [0]  setvar    : Type
 
 def e₁ :=
-  (lam (pi (fv 0) $ pi (fv 0) prop)
-    (for $ exi $ for $
-      (bin (bin (bv 0) mem (bv 1))
-       iff (bin (bin (bv 0) mem (bv 2))
-            and (app (app (bv 3) (bv 2)) (bv 0))))))
+  lam (pi (var 13) $ pi (var 13) prop) $
+    app (var 4) ∘ lam (var 14) $
+      app (var 4) ∘ lam (var 15) $
+        app (var 6) ∘ lam (var 16) $
+          (bin (bin (var 0) (var 4) (var 1))
+            (var 8) (bin (bin (var 0) (var 4) (var 2))
+              (var 11) (app (app (var 3) (var 2)) (var 0))))
 
 meta def main : io unit := do
 { io.put_str_ln c₁.to_string,
